WIP specification wp-rule IsUnique

theories/rules/rules_IsUnique.v
@@ -18,35 +18,144 @@ Section cap_lang_rules.
   Implicit Types mem : Mem.
   Implicit Types lmem : LMem.
 
+
+  Definition overlap_lwords (lw1 lw2 : LWord) : Prop :=
+    (overlap_word (lword_get_word lw1) (lword_get_word lw2)) = true.
+
+  (* For all addresses in the given region, update the version of the address *)
+  Definition update_version (lmem : LMem) (region : list Addr) (old_v new_v : Version)
+    : option LMem :=
+    foldl
+      (fun (opt_lmem' : option LMem) (a : Addr) =>
+         lmem' ← opt_lmem';
+         lw ← lmem' !! (a, old_v);
+         Some (<[(a, new_v) := lw ]> lmem'))
+      (Some lmem)
+      region.
+
+  (* Forall addresses a in the region, we update with v', if it exists a max_version mv st. *)
+  (* 1. lmem !! (a, mv) = lw  *)
+  (* 2. ∀ v. (∃ lw',  lmem !! (a, v) = lw') → v ≤ mv *)
+  (* 3. lmem' = <[ (a, v') = lw ]> lmem *)
+
+  (* Definition get_max_version (lmem : LMem) (a : Addr) : Version := *)
+ (*   map_fold *)
+  (*     (fun (la : LAddr) (_ : LWord) (max_version : Version) => *)
+  (*        if ((laddr_get_addr la) =? a)%a *)
+  (*        then max (laddr_get_version la) max_version *)
+  (*        else max_version) *)
+  (*     0 *)
+  (*     lmem. *)
+
+  (* TODO we don't need to get the max_version of an address, because *)
+  (* we already know, by construction, that we have the current view of the region *)
+  (* and that all addresses in the region also have the current version *)
+  Inductive IsUnique_spec
+    (lregs: LReg) (lmem : LMem) (dst src : RegName)
+    (lregs': LReg) (lmem' : LMem) : cap_lang.val → Prop :=
+
+  | IsUnique_success_true (lwsrc: LWord) p b e a v :
+    lregs !! src = Some lwsrc ->
+    get_lcap lwsrc = Some (LSCap p b e a v) ->
+    (* check if the words overlap only if the versions matches *)
+    Forall
+      (fun '(la, lw) => (laddr_get_version la) = v -> not (overlap_lwords lwsrc lw))
+      (map_to_list lmem) ->
+    (* we update the region of memory with the new version *)
+    update_version lmem (finz.seq_between b e) v (v + 1) = Some lmem' ->
+
+    incrementLPC (<[ dst := LInt 1 ]> (<[ src := LCap p b e a (v+1) ]> lregs)) = Some lregs' ->
+    IsUnique_spec lregs lmem dst src lregs' lmem' NextIV
+
+  | IsUnique_success_false (lwsrc: LWord) p b e a v :
+
+    lregs !! src = Some lwsrc ->
+    get_lcap lwsrc = Some (LSCap p b e a v) ->
+    (* it exists a word in the memory that overlaps somewhere in the memory *)
+    Exists
+      (fun '(la, lw) => (laddr_get_version la) = v -> overlap_lwords lwsrc lw)
+      (map_to_list lmem) ->
+    incrementLPC (<[ dst := LInt 0 ]> lregs) = Some lregs' ->
+    lmem' = lmem ->
+    IsUnique_spec lregs lmem dst src lregs' lmem' NextIV
+
+
+  | IsUnique_fail (lwsrc: LWord) :
+    lmem = lmem' → (* TODO are the equality condition actually necessary ? *)
+    lregs = lregs' →
+    lregs !! src = Some lwsrc ->
+    is_log_cap lwsrc = false →
+    IsUnique_spec lregs lmem dst src lregs' lmem' FailedV.
+
+
   (* TODO @Bastien *)
-  Lemma wp_isunique E pc_p pc_b pc_e pc_a pc_v pca_v lw dst src :
+
+  Definition allow_access_map_or_true (r : RegName) (lregs : LReg) (lmem : LMem) : Prop :=
+    exists p b e a v, read_reg_inr lregs r p b e a v
+                 ∧ if decide (lregs !! r = Some (LCap p b e a v))
+                   then Forall (fun a' => exists lw, lmem !! (a',v) = Some lw) (finz.seq_between b e)
+                   else True.
+
+  Lemma wp_isunique Ep
+    pc_p pc_b pc_e pc_a pc_v pca_v
+    (dst src : RegName) lw lmem lregs :
     decodeInstrWL lw = IsUnique dst src →
     isCorrectLPC (LCap pc_p pc_b pc_e pc_a pc_v) →
+    lregs !! PC = Some (LCap pc_p pc_b pc_e pc_a pc_v) →
+    regs_of (IsUnique dst src) ⊆ dom lregs →
+    lmem !! (pc_a, pca_v) = Some lw →
+    allow_access_map_or_true src lregs lmem →
 
-    {{{ PC ↦ᵣ LCap pc_p pc_b pc_e pc_a pc_v ∗ (pc_a, pca_v) ↦ₐ lw }}}
-      Instr Executable @ E
-    {{{ RET FailedV; PC ↦ᵣ LCap pc_p pc_b pc_e pc_a pc_v ∗ (pc_a, pca_v) ↦ₐ lw }}}.
+    {{{ (▷ [∗ map] la↦lw ∈ lmem, la ↦ₐ lw) ∗
+          ▷ [∗ map] k↦y ∈ lregs, k ↦ᵣ y }}}
+      Instr Executable @ Ep
+      {{{ lregs' lmem' retv, RET retv;
+          ⌜ IsUnique_spec lregs lmem dst src lregs' lmem' retv⌝ ∗
+            ([∗ map] la↦lw ∈ lmem', la ↦ₐ lw) ∗
+            [∗ map] k↦y ∈ lregs', k ↦ᵣ y }}}.
   Proof.
-    iIntros (Hinstr Hvpc φ) "[Hpc Hpca] Hφ".
+    iIntros (Hinstr Hvpc HPC Dregs Hmem_pc HaAccess φ) "(>Hmem & >Hmap) Hφ".
     apply isCorrectLPC_isCorrectPC_iff in Hvpc; cbn in Hvpc.
     iApply wp_lift_atomic_head_step_no_fork; auto.
     iIntros (σ1 ns l1 l2 nt) "Hσ1 /=". destruct σ1; simpl.
     iDestruct "Hσ1" as (lr lm cur_map) "(Hr & Hm & %HLinv)"; simpl in HLinv.
-    iDestruct (@gen_heap_valid with "Hr Hpc") as %?.
-    iDestruct (@gen_heap_valid with "Hm Hpca") as %?.
+
+    (* Derive necessary register values in r *)
+    iDestruct (gen_heap_valid_inclSepM with "Hr Hmap") as %Hregs.
+    have Hregs_pc := lookup_weaken _ _ _ _ HPC Hregs.
+    specialize (indom_lregs_incl _ _ _ Dregs Hregs) as Hri. unfold regs_of in Hri.
+    odestruct (Hri dst) as [ldstv [Hldst' Hldst]]. by set_solver+.
+    odestruct (Hri src) as [lsrcv [Hlsrc' Hlsrc]]. by set_solver+.
+
+    (* Derive necessary memory *)
+    iDestruct (gen_heap_valid_inclSepM with "Hm Hmem") as %Hmem.
+    iDestruct (gen_mem_valid_inSepM lmem lm with "Hm Hmem") as %Hma; eauto.
+
     iModIntro.
     iSplitR. by iPureIntro; apply normal_always_head_reducible.
-    iIntros (e2 σ2 efs Hstep).
-    apply prim_step_exec_inv in Hstep as (-> & -> & (c & -> & Hstep)).
-    iNext; iIntros "_".
-    iSplitR; auto. eapply step_exec_inv in Hstep; eauto.
-    2: eapply state_phys_log_reg_get_word in H2; eauto.
-    2: eapply state_phys_log_mem_get_word in H3; eauto.
-    cbn in Hstep; simplify_eq.
-    iModIntro.
-    iSplitR "Hφ Hpc Hpca"; last (iApply "Hφ" ; iFrame).
-    iExists lr, lm, cur_map.
-    iFrame; auto.
-   Qed.
+    iNext. iIntros (e2 σ2 efs Hpstep).
+    apply prim_step_exec_inv in Hpstep as (-> & -> & (c & -> & Hstep)).
+    iIntros "_".
+    iSplitR; auto; eapply step_exec_inv in Hstep; eauto.
+    2: eapply state_phys_corresponds_reg ; eauto ; cbn ; eauto.
+    2: eapply state_phys_corresponds_mem ; eauto; cbn ; eauto.
+
+
+    set (srcv := lword_get_word lsrcv).
+    assert ( reg !! src = Some srcv ) as Hsrc
+    by (eapply state_phys_log_reg_get_word ; eauto).
+    rewrite /exec /= Hsrc /= in Hstep.
+
+    (* Start the different cases now *)
+    destruct (is_log_cap lsrcv) eqn:Hlsrcv; cycle 1.
+    { (* Fail : not a capability *) admit.
+
+    }
+    subst srcv; cbn in *.
+    destruct_lword lsrcv; cbn in * ; try congruence. clear Hlsrcv.
+
+    admit.
+
+   Admitted.
 
 End cap_lang_rules.
